some inf' stuff

src/missing_mathlib/data/finset/lattice.lean
@@ -15,89 +15,7 @@ variables {s s₁ s₂ : finset β} {f : β → α}
 @[simp] lemma sup_cons {b : β} (h : b ∉ s) : (cons b s h).sup f = f b ⊔ s.sup f :=
 fold_cons h
 
-end sup
-
-section sup'
-variables [semilattice_sup α]
-
-theorem sup_of_mem {s : finset β} (f : β → α) {b : β} (h : b ∈ s) :
-  ∃ a, @sup (with_bot α) β _ s (some ∘ f) = some a :=
-(@le_sup (with_bot α) β _ s (some ∘ f) b h (f b) rfl).imp (fun b, Exists.fst)
-
-theorem le_sup_of_mem {s : finset β} (f : β → α) {b : β} (h : b ∈ s) {a : α}
-  (h₂ : @sup (with_bot α) β _ s (some ∘ f) = a) : f b ≤ a :=
-begin
-  rcases @le_sup (with_bot α) β _ s (some ∘ f) b h _ rfl with ⟨c, hb, ab⟩,
-  cases h₂.symm.trans hb,
-  assumption,
-end
-
-def sup' (s : finset β) (H : s.nonempty) (f : β → α) : α :=
-option.get $ let ⟨k, hk⟩ := H in option.is_some_iff_exists.2 (sup_of_mem f hk)
-
-theorem le_sup' {s : finset β} (f : β → α) {b : β} (H2 : b ∈ s) : f b ≤ s.sup' ⟨b, H2⟩ f :=
-le_sup_of_mem f H2 $ option.get_mem _
-
-theorem sup'_le {s : finset β} (H : s.nonempty) (f : β → α) {a : α} (H2 : ∀ b ∈ s, f b ≤ a) :
-  s.sup' H f ≤ a :=
-begin
-  rw [←with_bot.some_le_some, sup', option.some_get],
-  apply @sup_le (with_bot α) β _,
-  intros b hb,
-  rw with_bot.some_le_some,
-  exact H2 b hb,
-end
-
-variables {s : finset β} (H : s.nonempty) (f : β → α)
-
-@[simp] lemma coe_sup'_eq_sup : ((s.sup' H f : α) : with_bot α) = s.sup (coe ∘ f) :=
-by { rw [sup', ←with_bot.some_eq_coe, option.some_get], refl }
-
-lemma sup'_cons {b : β} (hb : b ∉ s) :
-  (cons b s hb).sup' (nonempty_cons hb) f = f b ⊔ s.sup' H f :=
-by { rw ←with_bot.coe_eq_coe, simp }
-
-lemma sup'_insert [decidable_eq β] {b : β} (h : (insert b s).nonempty) :
-  (insert b s).sup' h f = f b ⊔ s.sup' H f :=
-by { rw ←with_bot.coe_eq_coe, simp }
-
-end sup'
-
-section sup
-variables {C : β → Type*} [∀ (b : β), semilattice_sup_bot (C b)]
-
-protected lemma sup_apply (s : finset α) (f : α → ∀ (b : β), C b) (b : β) :
-  s.sup f b = s.sup (fun a, f a b) :=
-begin
-  induction s using finset.induction' with c s hc ih,
-  { refl, },
-  { rw [sup_cons, sup_cons, sup_apply, ih], },
-end
-
-end sup
-
-section sup'
-variables [decidable_eq α] {C : β → Type*} [∀ (b : β), semilattice_sup (C b)]
-
-lemma sup'_apply {s : finset α} (h : s.nonempty) (f : α → ∀ (b : β), C b) (b : β) :
-  s.sup' h f b = s.sup' h (fun a, f a b) :=
-begin
-  induction s using finset.induction_on with c s hc ih,
-  { exfalso,
-    exact not_nonempty_empty h, },
-  { cases dec_em (s = ∅) with he hne,
-    { subst he,
-      refl, },
-    { repeat { rw sup'_insert (nonempty_of_ne_empty hne), },
-      rw [sup_apply, ih], }, },
-end
-
-end sup'
-
-section sup
-variables [semilattice_sup_bot α]
-
-lemma of_sup_of_forall {s : finset β} (f : β → α) {p : α → Prop} (h0 : p ⊥)
+lemma of_sup_of_forall {p : α → Prop} (h0 : p ⊥)
   (hp : ∀ (a₁ a₂ : α), p a₁ → p a₂ → p (a₁ ⊔ a₂)) (hs : ∀ b ∈ s, p (f b)) : p (s.sup f) :=
 begin
   induction s using finset.induction' with c s hc ih,
@@ -116,20 +34,149 @@ end
 
 end sup
 
+section inf
+variables [semilattice_inf_top α]
+
+variables {s s₁ s₂ : finset β} {f : β → α}
+
+@[simp] lemma inf_cons {b : β} (h : b ∉ s) : (cons b s h).inf f = f b ⊓ s.inf f :=
+@sup_cons (order_dual α) _ _ _ _ _ h
+
+lemma of_inf_of_forall {p : α → Prop} (h0 : p ⊤)
+  (hp : ∀ (a₁ a₂ : α), p a₁ → p a₂ → p (a₁ ⊓ a₂)) (hs : ∀ b ∈ s, p (f b)) : p (s.inf f) :=
+@of_sup_of_forall (order_dual α) _ _ _ _ _ h0 hp hs
+
+end inf
+
+section sup'
+variables [semilattice_sup α]
+
+lemma sup_of_mem {s : finset β} (f : β → α) {b : β} (h : b ∈ s) :
+  ∃ (a : α), @sup (with_bot α) _ _ s (coe ∘ f) = ↑a :=
+(@le_sup (with_bot α) _ _ _ _ _ h (f b) rfl).imp (fun b, Exists.fst)
+
+lemma le_sup_of_mem {s : finset β} (f : β → α) {b : β} (h₁ : b ∈ s) {a : α}
+  (h₂ : @sup (with_bot α) _ _ s (coe ∘ f) = ↑a) : f b ≤ a :=
+begin
+  rcases @le_sup (with_bot α) _ _ _ _ _ h₁ (f b) rfl with ⟨c, hb, ab⟩,
+  cases h₂.symm.trans hb,
+  assumption,
+end
+
+def sup' (s : finset β) (H : s.nonempty) (f : β → α) : α :=
+option.get $ let ⟨k, hk⟩ := H in option.is_some_iff_exists.2 (sup_of_mem f hk)
+
+@[simp] lemma coe_sup'_eq_sup_coe {s : finset β} (H : s.nonempty) (f : β → α) :
+  ((s.sup' H f : α) : with_bot α) = s.sup (coe ∘ f) :=
+by rw [sup', ←with_bot.some_eq_coe, option.some_get]
+
+lemma le_sup' {s : finset β} (f : β → α) {b : β} (H2 : b ∈ s) : f b ≤ s.sup' ⟨b, H2⟩ f :=
+le_sup_of_mem f H2 $ option.get_mem _
+
+lemma sup'_le {s : finset β} (H : s.nonempty) (f : β → α) {a : α} (H2 : ∀ b ∈ s, f b ≤ a) :
+  s.sup' H f ≤ a :=
+begin
+  rw [←with_bot.coe_le_coe, coe_sup'_eq_sup_coe],
+  apply @sup_le (with_bot α) β _,
+  intros b hb,
+  rw with_bot.coe_le_coe,
+  exact H2 b hb,
+end
+
+variables {s : finset β} (H : s.nonempty) (f : β → α)
+
+lemma sup'_cons {b : β} (hb : b ∉ s) :
+  (cons b s hb).sup' (nonempty_cons hb) f = f b ⊔ s.sup' H f :=
+by { rw ←with_bot.coe_eq_coe, simp }
+
+lemma sup'_insert [decidable_eq β] {b : β} (h : (insert b s).nonempty) :
+  (insert b s).sup' h f = f b ⊔ s.sup' H f :=
+by { rw ←with_bot.coe_eq_coe, simp }
+
+end sup'
+
+section inf'
+variable [semilattice_inf α]
+
+lemma inf_of_mem {s : finset β} (f : β → α) {b : β} (h : b ∈ s) :
+  ∃ (a : α), @inf (with_top α) _ _ s (coe ∘ f) = ↑a :=
+@sup_of_mem (order_dual α) _ _ _ _ _ h
+
+lemma inf_le_of_mem {s : finset β} (f : β → α) {b : β} (h₁ : b ∈ s) {a : α}
+  (h₂ : @inf (with_top α) _ _ s (coe ∘ f) = ↑a) : a ≤ f b :=
+@le_sup_of_mem (order_dual α) _ _ _ _ _ h₁ _ h₂
+
+def inf' (s : finset β) (H : s.nonempty) (f : β → α) : α :=
+@sup' (order_dual α) _ _ s H f
+
+@[simp] lemma coe_inf'_eq_inf_coe {s : finset β} (H : s.nonempty) (f : β → α) :
+  ((s.inf' H f : α) : with_top α) = s.inf (coe ∘ f) :=
+@coe_sup'_eq_sup_coe (order_dual α) _ _ _ H f
+
+end inf'
+
+section sup
+variables {C : β → Type*} [Π (b : β), semilattice_sup_bot (C b)]
+
+protected lemma sup_apply (s : finset α) (f : α → Π (b : β), C b) (b : β) :
+  s.sup f b = s.sup (fun a, f a b) :=
+begin
+  induction s using finset.induction' with c s hc ih,
+  { refl, },
+  { rw [sup_cons, sup_cons, sup_apply, ih], },
+end
+
+end sup
+
+section inf
+variables {C : β → Type*} [Π (b : β), semilattice_inf_top (C b)]
+
+protected lemma inf_apply (s : finset α) (f : α → Π (b : β), C b) (b : β) :
+  s.inf f b = s.inf (fun a, f a b) :=
+@finset.sup_apply _ _ (fun b, order_dual (C b)) _ _ _ _
+
+end inf
+
+section sup'
+variables [decidable_eq α] {C : β → Type*} [Π (b : β), semilattice_sup (C b)]
+
+lemma sup'_apply {s : finset α} (h : s.nonempty) (f : α → Π (b : β), C b) (b : β) :
+  s.sup' h f b = s.sup' h (fun a, f a b) :=
+begin
+  induction s using finset.induction_on with c s hc ih,
+  { exfalso,
+    exact not_nonempty_empty h, },
+  { cases dec_em (s = ∅) with he hne,
+    { subst he,
+      refl, },
+    { repeat { rw sup'_insert (nonempty_of_ne_empty hne), },
+      rw [sup_apply, ih], }, },
+end
+
+end sup'
+
+section inf'
+variables [decidable_eq α] {C : β → Type*} [Π (b : β), semilattice_inf (C b)]
+
+lemma inf'_apply {s : finset α} (h : s.nonempty) (f : α → Π (b : β), C b) (b : β) :
+  s.inf' h f b = s.inf' h (fun a, f a b) :=
+@sup'_apply _ _ _ (fun b, order_dual (C b)) _ _ _ _ _
+
+end inf'
+
 section sup'
 variable [semilattice_sup α]
 
-lemma of_sup'_of_forall {s : finset β} (hne : s.nonempty) (f : β → α) {p : α → Prop}
+lemma of_sup'_of_forall {s : finset β} (hne : s.nonempty) {f : β → α} {p : α → Prop}
   (hp : ∀ (a₁ a₂ : α), p a₁ → p a₂ → p (a₁ ⊔ a₂)) (hs : ∀ b ∈ s, p (f b)) : p (s.sup' hne f) :=
 begin
   cases hne with k hk,
   cases sup_of_mem f hk with m hm,
   rw show s.sup' ⟨k, hk⟩ f = m,
-  { rwa [←with_bot.coe_eq_coe, coe_sup'_eq_sup], },
-  let p' := @option.rec α (fun _, Prop) true p,
-  change p' (some m),
+  { rwa [←with_bot.coe_eq_coe, coe_sup'_eq_sup_coe], },
+  change @option.rec α (fun _, Prop) true p ↑m,
   rw ←hm,
-  refine of_sup_of_forall (coe ∘ f) trivial _ hs,
+  refine of_sup_of_forall trivial _ hs,
   intros a₁ a₂ h₁ h₂,
   cases a₁,
   { rwa [with_bot.none_eq_bot, bot_sup_eq], },
@@ -139,5 +186,14 @@ begin
 end
 
 end sup'
+
+section inf'
+variable [semilattice_inf α]
+
+lemma of_inf'_of_forall {s : finset β} (hne : s.nonempty) {f : β → α} {p : α → Prop}
+  (hp : ∀ (a₁ a₂ : α), p a₁ → p a₂ → p (a₁ ⊓ a₂)) (hs : ∀ b ∈ s, p (f b)) : p (s.inf' hne f) :=
+@of_sup'_of_forall (order_dual α) _ _ _ _ _ _ hp hs
+
+end inf'
 
 end finset
